update passwordCheck_safe and outline

timing/examples/FreeRTOS/queue/uxQueueSpacesAvailable.v
@@ -6,7 +6,7 @@ Import RISCVNotations.
 
 Module TimingProof (cpu : CPUTimingBehavior).
 
-Module Program_xQueueMessagesWaiting <: ProgramInformation.
+Module Program_uxQueueSpacesAvailable <: ProgramInformation.
     Definition entry_addr : N := 0x80003590.
 
     Definition exits (t:trace) : bool :=
@@ -16,14 +16,14 @@ Module Program_xQueueMessagesWaiting <: ProgramInformation.
     end | _ => false end.
 
     Definition binary := RTOSDemo.
-End Program_xQueueMessagesWaiting.
+End Program_uxQueueSpacesAvailable.
 
-Module RISCVTiming := RISCVTiming cpu Program_xQueueMessagesWaiting.
-Module xQueueMessagesWaitingAuto := RISCVTimingAutomation RISCVTiming.
-Import Program_xQueueMessagesWaiting xQueueMessagesWaitingAuto.
+Module RISCVTiming := RISCVTiming cpu Program_uxQueueSpacesAvailable.
+Module uxQueueSpacesAvailableAuto := RISCVTimingAutomation RISCVTiming.
+Import Program_uxQueueSpacesAvailable uxQueueSpacesAvailableAuto.
 
 (* Postcondition *)
-Definition time_of_xQueueMessagesWaiting (t : trace) (mem : memory) :=
+Definition time_of_uxQueueSpacesAvailable (t : trace) (mem : memory) :=
     cycle_count_of_trace t =
         tcsrrci + tlw + tlw + tsub + tlui + tlw +
         if (mem Ⓓ[0x80080004] =? 0) then (
@@ -33,24 +33,24 @@ Definition time_of_xQueueMessagesWaiting (t : trace) (mem : memory) :=
         ) + tjalr.
 
 (* Invariants *)
-Definition xQueueMessagesWaiting_timing_invs (base_mem : memory)
+Definition uxQueueSpacesAvailable_timing_invs (base_mem : memory)
     (t:trace) : option Prop :=
 match t with (Addr a, s) :: t' => match a with
 | 0x80003590 => Some (s V_MEM32 = base_mem /\
             cycle_count_of_trace t' = 0)
-| 0x800035b0 | 0x800029ac => Some (time_of_xQueueMessagesWaiting t base_mem)
+| 0x800035b0 | 0x800029ac => Some (time_of_uxQueueSpacesAvailable t base_mem)
 | _ => None end | _ => None end.
 
 (*step through tactics in psimpl_in_hyp*)
 
-Theorem xQueueMessagesWaiting_timing:
+Theorem uxQueueSpacesAvailable_timing:
   forall s t s' x' base_mem
          (ENTRY: startof t (x',s') = (Addr entry_addr, s))
          (MDL: models rvtypctx s)
          (MEM: s V_MEM32 = base_mem),
   satisfies_all 
     lifted_prog
-    (xQueueMessagesWaiting_timing_invs base_mem)
+    (uxQueueSpacesAvailable_timing_invs base_mem)
     exits
   ((x',s')::t).
 Proof using.
