timing/examples/crypto/passwordCheck/passwordCheck_safe_proofs.v
@@ -31,34 +31,29 @@ Lemma le_cases : forall n m,
     n <= m -> n < m \/ n = m.
 Proof. lia. Qed.
 
-Definition time_of_passwordCheck (len_stored len_user : N) (t : trace) :=
+Definition time_of_passwordCheck (len_user : N) (t : trace) :=
     cycle_count_of_trace t =
         taddi +
-        (N.min len_stored len_user) * (
-            tlbu + tlbu + taddi + tsltiu + tsub + tsltiu +
-            tor + tand + taddi + tfbeq + ttbne
-        ) + (tlbu + tlbu + taddi + tsltiu + tsub + tsltiu +
-            tor + tand + taddi) + 
-        (if len_user <=? len_stored then (
-            ttbeq
-        ) else (
-            tfbeq + tfbne
-        )) + taddi + tandi + tjalr.
+        len_user * (
+            tlbu + tlbu + tsub + tsltiu + tsltiu +
+            tor + tand + taddi + tsltu + tadd + ttbne
+        ) + tlbu + tlbu + tsub + tsltiu + tsltiu +
+            tor + tand + taddi + tsltu + tadd + tfbne +
+        taddi + tandi + tjalr.
 
 Definition passwordCheck_timing_invs (s : store) (base_mem : memory)
-    (stored user : addr) (len1 len2 : N) (t:trace) : option Prop :=
+    (stored user : addr) (user_len : N) (t:trace) : option Prop :=
 match t with (Addr a, s) :: t' => match a with
 | 0x1e8 => Some (
     exists i,
+    i <= user_len /\
     s V_MEM32 = base_mem /\ s R_A0 = stored ⊕ i /\ s R_A1 = user ⊕ i /\
-    i <= N.min len1 len2 /\
-    strlen base_mem stored len1 /\
-    strlen base_mem user len2 /\
+    strlen base_mem user user_len /\
     cycle_count_of_trace t' = taddi +
-        i * (tlbu + tlbu + taddi + tsltiu + tsub + tsltiu +
-            tor + tand + taddi + tfbeq + ttbne)
+        i * (tlbu + tlbu + tsub + tsltiu + tsltiu +
+            tor + tand + taddi + tsltu + tadd + ttbne)
 )
-| 0x21c => Some (time_of_passwordCheck len1 len2 t)
+| 0x21c => Some (time_of_passwordCheck user_len t)
 | _ => None end | _ => None end.
 
 Lemma strlen_Sidx_le_len : forall i len mem p,
@@ -86,19 +81,18 @@ Proof.
 Qed.
 
 Theorem passwordCheck_timing:
-  forall s (t : trace) s' x' base_mem stored user len1 len2
+  forall s (t : trace) s' x' base_mem stored user user_len
          (* boilerplate *)
          (ENTRY: startof t (x',s') = (Addr entry_addr, s))
          (MDL: models rvtypctx s)
          (* bindings *)
          (MEM: s V_MEM32 = base_mem)
-         (LEN1: strlen base_mem stored len1)
-         (LEN2: strlen base_mem user len2)
+         (ULEN: strlen base_mem user user_len)
          (Stored: s R_A0 = stored)
          (User: s R_A1 = user),
   satisfies_all 
     lifted_prog
-    (passwordCheck_timing_invs s base_mem stored user len1 len2)
+    (passwordCheck_timing_invs s base_mem stored user user_len)
     exits
   ((x',s')::t).
 Proof using.
@@ -107,13 +101,8 @@ Proof using.
     Local Ltac step := tstep r5_step.
 
     simpl. rewrite ENTRY. unfold entry_addr. step.
-    exists 0. repeat split; try lia; try apply LEN1; try apply LEN2.
-    1-2: (rewrite N.add_0_r, N.mod_small; [assumption|subst]).
-    pose proof (models_var R_A0 MDL) as H; simpl in H.
-        apply H.
-    pose proof (models_var R_A1 MDL) as H; simpl in H.
-        apply H.
-    hammer.
+    exists 0.
+    psimpl. repeat (split; auto; lia).
 
     intros.
     eapply startof_prefix in ENTRY; try eassumption.
@@ -123,47 +112,23 @@ Proof using.
 
     destruct_inv 32 PRE.
 
-    destruct PRE as (i & MEM & A0 & A1 & ILen & Strlen1 & Strlen2 &
-                        Cycles).
+    destruct PRE as (i & ILEN & MEM & A0 & A1 & Strlen & Cycles).
     repeat step.
-    - (* user[i] = NULL *)
-        hammer. apply N.min_glb_iff in ILen.
-        destruct ILen.
-        pose proof (strlen_idx_eq_len i 
-            len2 base_mem user H0 Strlen2 BC). subst.
-        rewrite (N.min_r _ _ H).
-        destruct (N.eq_dec len2 len1).
-            subst. rewrite N.leb_refl. lia.
-        replace (len2 <=? len1) with true. lia.
-        symmetry. now apply N.leb_le in H.
-    -(* user[i] <> NULL, stored[i] <> NULL *)
-        apply N.min_glb_iff in ILen.
-        apply Bool.negb_true_iff in BC0.
-        destruct ILen.
-        pose proof (strlen_Sidx_le_len i
-            len1 base_mem stored H Strlen1 BC0).
-        pose proof (strlen_Sidx_le_len i
-            len2 base_mem user H0 Strlen2 BC).
-        exists (i + 1). psimpl.
-        split. reflexivity.
-        split. reflexivity.
-        split. reflexivity.
-        split. now apply N.min_glb.
-        split. assumption.
-        split. assumption.
+    - (* user[i] <> NULL *)
+        exists (1 + i). repeat (split; auto).
+        apply Bool.negb_true_iff in BC.
+            eapply strlen_Sidx_le_len; eauto.
+        now psimpl.
+        apply Bool.negb_true_iff in BC.
+            replace (0 <? _) with true by lia. now psimpl.
         hammer.
-    - (* user[i] <> NULL, stored[i] = NULL *)
-        hammer. apply N.min_glb_iff in ILen.
-        destruct ILen.
-        apply Bool.negb_false_iff in BC0.
-        pose proof (strlen_idx_eq_len i 
-            len1 base_mem stored H Strlen1 BC0). subst.
-        pose proof (strlen_Sidx_le_len len1
-            len2 (s' V_MEM32) user ltac:(lia) Strlen2 BC).
-        assert (len1 < len2) by lia.
-        replace (len2 <=? len1) with false.
-        rewrite (N.min_l _ _ H0). lia.
-        symmetry. apply N.leb_gt. assumption.
+    - (* user[i] = NULL *)
+        hammer.
+        destruct Strlen.
+        rewrite (strlen_idx_eq_len i user_len base_mem user).
+            lia.
+        assumption. now split.
+        now apply Bool.negb_false_iff in BC.
 Qed.
 
 End TimingProof.
